grind

src/Pipit.Exec.Exp.fst
@@ -8,54 +8,59 @@ open Pipit.Exp.Base
 module C  = Pipit.Context.Base
 module CR = Pipit.Context.Row
 
-let row_cons (#a: eqtype) (#c: context 't) (v: a) (values: row c): row (C.lift1 c 0 'a) = (v, values)
+let row_cons (#t: table) (#c: context t) (#a: t.ty) (v: t.ty_sem a) (values: row c): row (C.lift1 c 0 a) = (v, values)
 
-let exec_index (c: C.context) (ix: C.index { C.has_index c ix }):
-       exec (C.row c) unit (List.Tot.index c ix) =
+let exec_index (#t: table) (c: context t) (ix: C.index_lookup c):
+       exec (row c) unit (List.Tot.index (context_sem c) ix) =
   { init = ()
-  ; eval = (fun i s -> C.row_index c i ix)
+  ; eval = (fun i s -> CR.index (context_sem c) i ix)
   ; update = (fun i s -> ())
   }
 
-let rec state_of_exp (e: exp 'c 'a): Tot Type (decreases e) =
+[@@strict_on_arguments [2]]
+let rec state_of_exp (#t: table) (#c: context t) (e: exp t c 'a): Tot Type (decreases e) =
   match e with
   | XVal v -> unit
+  | XPrim p -> unit
   | XBVar x -> unit
   | XVar x -> unit
   | XApp f e -> state_of_exp f & state_of_exp e
   | XFby v e -> state_of_exp e & 'a
   | XThen e1 e2 -> bool & state_of_exp e2
-  | XMu _ e1 -> state_of_exp e1
+  | XMu e1 -> state_of_exp e1
   | XLet b e1 e2 -> state_of_exp e1 & state_of_exp e2
   // | XContract assm guar body arg -> unit
   | XCheck p e1 e2 -> state_of_exp e2
 
-let xexec (e: exp 'c 'a) = exec (C.row 'c) (state_of_exp e) 'a
+let xexec (#t: table) (#c: context t) (e: exp t c 'a) = exec (row c) (state_of_exp e) 'a
 
-let rec extractable (e: exp 'c 'a): Tot prop (decreases e) =
+let rec extractable (#t: table) (#c: context t) (e: exp t c 'a): Tot prop (decreases e) =
   match e with
   | XVal v -> True
+  | XPrim p -> True
   | XBVar i -> True
   | XVar x -> False
   | XApp e1 e2 -> extractable e1 /\ extractable e2
   | XFby v e1 -> extractable e1
   | XThen e1 e2 -> extractable e1 /\ extractable e2
-  | XMu _ e1 ->
+  | XMu e1 ->
     extractable e1
   | XLet b e1 e2 -> extractable e1 /\ extractable e2
   // | XContract assm guar body arg -> False
   | XCheck p e1 e2 -> extractable e2
 
-let extractable_XApp (e1: exp 'c ('b -> 'a)) (e2: exp 'c 'b):
+let extractable_XApp (#t: table) (#c: context t) (e1: exp t c ('b -> 'a)) (e2: exp t c 'b):
   Lemma (requires (extractable (XApp e1 e2)))
         (ensures (extractable e1)) =
         assert_norm (extractable (XApp e1 e2) ==> extractable e1)
 
+[@@strict_on_arguments [2]]
 noextract inline_for_extraction
-let rec exec_of_exp (e: exp 't 'c 'a { extractable e }): Tot (xexec e) (decreases e) =
+let rec exec_of_exp (#t: table) (#c: context t) (e: exp t c 'a { extractable e }): Tot (xexec e) (decreases e) =
   match e with
   | XVal v -> exec_const _ v
-  | XBVar i -> exec_index 'c i
+  | XPrim p -> exec_const _ (t.prim_sem p)
+  | XBVar i -> exec_index c i
   // | XVar x ->
   | XApp e1 e2 ->
     extractable_XApp e1 e2;
@@ -67,8 +72,8 @@ let rec exec_of_exp (e: exp 't 'c 'a { extractable e }): Tot (xexec e) (decrease
     exec_pre v (exec_of_exp e1)
   | XThen e1 e2 ->
     exec_then (exec_of_exp e1) (exec_of_exp e2)
-  | XMu i e1 ->
-    exec_mu (('t).val_default 'a) (fun i v -> row_cons v i) (exec_of_exp e1)
+  | XMu e1 ->
+    exec_mu (t.val_default (XMu?.valty e)) (fun i v -> row_cons v i) (exec_of_exp e1)
   | XLet b e1 e2 ->
     exec_let (fun i v -> row_cons v i) (exec_of_exp e1) (exec_of_exp e2)
   // | XContract assm guar body arg ->
