src/Pipit.System.Exp.fst
@@ -12,83 +12,89 @@ open Pipit.System.Det
 
 
 (* A system we get from translating an expression *)
-let xsystem (c: context) (state: Type) (value: Type) = system (row c) state value
+let xsystem (#t: table) (c: context t) (state: Type) (value: Type) = system (row c) state value
 (* Same, but deterministic *)
-let xdsystem (c: context) (state: Type) (value: Type) = dsystem (row c) state value
+let xdsystem (#t: table) (c: context t) (state: Type) (value: Type) = dsystem (row c) state value
 
 let xsystem_stepn
-  (#c: context)
+  (#tbl: table)
+  (#c: context tbl)
   (#state #value: Type)
   (t: xsystem c state value)
   (streams: list (row c & value))
   (s': state): prop =
   system_stepn t streams s'
 
-let rec state_of_exp (e: exp 'c 'a): Tot Type (decreases e) =
+let rec state_of_exp (#t: table) (#c: context t) (e: exp t c 'a): Tot Type (decreases e) =
   match e with
   | XVal v -> unit
+  | XPrim p -> unit
   | XBVar x -> unit
   | XVar x -> unit
   | XApp f e -> state_of_exp f & state_of_exp e
   | XFby v e1 -> state_of_exp e1 & 'a
   | XThen e1 e2 -> system_then_state (state_of_exp e1) (state_of_exp e2)
-  | XMu _ e1 -> state_of_exp e1
+  | XMu e1 -> state_of_exp e1
   | XLet b e1 e2 -> state_of_exp e1 & state_of_exp e2
   // Contracts do not expose their body, so we only need state of assumptions, guarantee and arg
   // | XContract assm guar body arg ->
   //   state_of_exp assm &
   //   state_of_exp guar &
   //   state_of_exp arg
-  | XCheck name e1 e2 -> (xprop & state_of_exp e1) & state_of_exp e2
+  | XCheck name e1 e2 -> (t.ty_sem t.propty & state_of_exp e1) & state_of_exp e2
 
-let rec dsystem_of_exp (e: exp 'c 'a { Causal.causal e }):
-    Tot (xdsystem 'c (state_of_exp e) 'a) (decreases e) =
+let rec dsystem_of_exp (#t: table) (#c: context t) (e: exp t c 'a { Causal.causal e }):
+    Tot (xdsystem c (state_of_exp e) 'a) (decreases e) =
   match e with
   | XVal v -> dsystem_const v
-  | XBVar x -> dsystem_map (fun i -> CR.index 'c i x) dsystem_input
+  | XPrim p -> dsystem_const (t.prim_sem p)
+  | XBVar x -> dsystem_map (fun i -> CR.index (context_sem c) i x) dsystem_input
   | XVar x -> false_elim ()
   | XApp e1 e2 ->
     assert_norm (Causal.causal (XApp e1 e2) ==> (Causal.causal e1 && Causal.causal e2));
     let t1 = dsystem_of_exp e1 in
     let t2 = dsystem_of_exp e2 in
-    let t': xdsystem 'c (state_of_exp (XApp e1 e2)) 'a = dsystem_ap2 t1 t2 in
+    let t': xdsystem c (state_of_exp (XApp e1 e2)) 'a = dsystem_ap2 t1 t2 in
     t'
   | XFby v e1 ->
     dsystem_pre v (dsystem_of_exp e1)
   | XThen e1 e2 ->
     dsystem_then (dsystem_of_exp e1) (dsystem_of_exp e2)
-  | XMu _ e1 ->
-    let t = dsystem_of_exp e1 in
-    dsystem_mu_causal #(row 'c) #('a & row 'c) (fun i v -> (v, i)) t
+  | XMu e1 ->
+    let t' = dsystem_of_exp e1 in
+    dsystem_mu_causal #(row c) #('a & row c) (t.val_default (XMu?.valty e)) (fun i v -> (v, i)) t'
   | XLet b e1 e2 ->
     dsystem_let (fun i v -> (v, i)) (dsystem_of_exp e1) (dsystem_of_exp e2)
   | XCheck name e1 e2 ->
-    let t1 = dsystem_check name (dsystem_of_exp e1) in
+    let t1 = dsystem_check t.propty_sem (t.propty_of_bool true) name (dsystem_of_exp e1) in
     let t2 = dsystem_of_exp e2 in
-    let t': xdsystem 'c (state_of_exp (XCheck name e1 e2)) 'a = dsystem_let (fun i v -> i) t1 t2 in
+    let t': xdsystem c (state_of_exp (XCheck name e1 e2)) 'a = dsystem_let (fun i v -> i) t1 t2 in
     t'
 
-let rec system_of_exp_rel (e: exp 'c 'a { Causal.causal e }):
-    Tot (xsystem 'c (state_of_exp e) 'a) (decreases e) =
+let rec system_of_exp_rel
+  (#t: table) (#c: context t)
+  (e: exp t c 'a { Causal.causal e }):
+    Tot (xsystem c (state_of_exp e) 'a) (decreases e) =
   // if exp_is_function e then system_of_dsystem (dsystem_of_exp e)
   // else
     match e with
     | XVal v -> system_const v
-    | XBVar x -> system_map (fun i -> CR.index 'c i x) system_input
+    | XPrim p -> system_const (t.prim_sem p)
+    | XBVar x -> system_map (fun i -> CR.index (context_sem c) i x) system_input
     | XVar x -> false_elim ()
     | XApp e1 e2 ->
       assert_norm (Causal.causal (XApp e1 e2) ==> (Causal.causal e1 && Causal.causal e2));
       let t1 = system_of_exp_rel e1 in
       let t2 = system_of_exp_rel e2 in
-      let t': xsystem 'c (state_of_exp (XApp e1 e2)) 'a = system_ap2 t1 t2 in
+      let t': xsystem c (state_of_exp (XApp e1 e2)) 'a = system_ap2 t1 t2 in
       t'
     | XFby v e1 ->
       system_pre v (system_of_exp_rel e1)
     | XThen e1 e2 ->
       system_then (system_of_exp_rel e1) (system_of_exp_rel e2)
-    | XMu _ e1 ->
-      let t = system_of_exp_rel e1 in
-      system_mu #(row 'c) #('a & row 'c) (fun i v -> (v, i)) t
+    | XMu e1 ->
+      let t' = system_of_exp_rel e1 in
+      system_mu #(row c) #('a & row c) (fun i v -> (v, i)) t'
     | XLet b e1 e2 ->
       system_let (fun i v -> (v, i)) (system_of_exp_rel e1) (system_of_exp_rel e2)
     // | XContract assm guar body arg ->
@@ -97,10 +103,10 @@ let rec system_of_exp_rel (e: exp 'c 'a { Causal.causal e }):
     //     (system_bool_holds (system_of_exp_rel guar))
     //     (system_of_exp_rel arg)
     | XCheck name e1 e2 ->
-      let t1 = system_check name (system_of_exp_rel e1) in
+      let t1 = system_check t.propty_sem (t.propty_of_bool true) name (system_of_exp_rel e1) in
       let t2 = system_of_exp_rel e2 in
-      let t': xsystem 'c (state_of_exp (XCheck name e1 e2)) 'a = system_let (fun i v -> i) t1 t2 in
+      let t': xsystem c (state_of_exp (XCheck name e1 e2)) 'a = system_let (fun i v -> i) t1 t2 in
       t'
 
-let system_of_exp (e: exp 'c 'a { Causal.causal e }) =
+let system_of_exp (#t: table) (#c: context t) (e: exp t c 'a { Causal.causal e }) =
   system_of_dsystem (dsystem_of_exp e)
