example/Simple.Check.fst
@@ -22,14 +22,14 @@ let count_when (p: s bool): s int =
    fby 0 count +^ (if_then_else p z1 z0))
 
 (* forall e. count_when false <= count_when e <= count_when true *)
-let count_when_prop (e: s bool): s unit =
-  let' (count_when ff) (fun count_when_false ->
-  let' (count_when  e) (fun count_when_e ->
-  let' (count_when tt) (fun count_when_true ->
+let count_when_prop (e: s bool): s bool =
+  let' #_ #bool (count_when ff) (fun count_when_false ->
+  let' #_ #bool (count_when  e) (fun count_when_e ->
+  let' #_ #bool (count_when tt) (fun count_when_true ->
   check' "0                <= count_when false" (z0               <=^ count_when_false) (
   check' "count_when false <= count_when e"     (count_when_false <=^ count_when_e) (
   check' "count_when e     <= count_when true"  (count_when_e     <=^ count_when_true) (
-  pure ()))))))
+  pure true))))))
 
 let sys =
   assert_norm (Pipit.Exp.Causality.causal (run1 count_when_prop));
