src/Pipit.Prim.Vanilla.fst
@@ -139,5 +139,6 @@ let table: table = {
    val_default = val_default;
 
    propty      = TBool;
-   propty_sem  = fun (x: bool) -> x == true
+   propty_sem  = (fun (x: bool) -> x == true);
+   propty_of_bool = (fun (x: bool) -> x);
 }
